theories/heap_lang/lib/ticket_lock.v
@@ -69,6 +69,16 @@ Section proof.
     iDestruct (own_valid_2 with "H1 H2") as %[[] _].
   Qed.
 
+  Lemma is_lock_iff γ lk R1 R2 :
+    is_lock γ lk R1 -∗ ▷ □ (R1 ↔ R2) -∗ is_lock γ lk R2.
+  Proof.
+    iDestruct 1 as (lo ln ->) "#Hinv"; iIntros "#HR".
+    iExists lo, ln; iSplit; [done|]. iApply (inv_iff with "Hinv").
+    iIntros "!> !#"; iSplit; iDestruct 1 as (o n) "(Ho & Hn & H● & H)";
+      iExists o, n; iFrame "Ho Hn H●";
+      (iDestruct "H" as "[[H◯ H]|H◯]"; [iLeft; iFrame "H◯"; by iApply "HR"|by iRight]).
+  Qed.
+
   Lemma newlock_spec (R : iProp Σ) :
     {{{ R }}} newlock #() {{{ lk γ, RET lk; is_lock γ lk R }}}.
   Proof.
@@ -162,5 +172,6 @@ End proof.
 Typeclasses Opaque is_lock issued locked.
 
 Canonical Structure ticket_lock `{!heapG Σ, !tlockG Σ} : lock Σ :=
-  {| lock.locked_exclusive := locked_exclusive; lock.newlock_spec := newlock_spec;
+  {| lock.locked_exclusive := locked_exclusive; lock.is_lock_iff := is_lock_iff;
+     lock.newlock_spec := newlock_spec;
      lock.acquire_spec := acquire_spec; lock.release_spec := release_spec |}.
